Add data types with constructors
This mostly recycles code from the data branch
where I used lists for applied constructors

Syntax.thy
@@ -5,41 +5,71 @@ begin
 atom_decl "var"
 atom_decl "tyvar"
 
+atom_decl "data_name"
+atom_decl "ctor_name"
+
 nominal_datatype "\<kappa>" =
   Star ("\<star>")
-  | KArrow "\<kappa>" "\<kappa>"
+  | KArrow "\<kappa>" "\<kappa>" (infixr "\<rightarrow>" 50)
 
 nominal_datatype "\<tau>" =
-  TyUnit
-  | TyVar "tyvar"
-  | TyArrow "\<tau>" "\<tau>"  ("_ \<rightarrow> _" 50)
-  | TyConApp "\<tau>" "\<tau>"
+  TyVar "tyvar"
+  | TyData "data_name"
+  | TyArrow
+  | TyApp "\<tau>" "\<tau>"
   | TyForall a::"tyvar" "\<kappa>" t::"\<tau>" binds a in t ("\<forall> _ : _ . _" 50)
+
+abbreviation arrow_app :: "\<tau> \<Rightarrow> \<tau> \<Rightarrow> \<tau>" (infixr "\<rightarrow>" 50) where
+  "arrow_app \<tau>1 \<tau>2 \<equiv> TyApp (TyApp TyArrow \<tau>1) \<tau>2"
 
 nominal_datatype "term" =
    Var "var"
  | App "term" "term"
- | TyApp "term" "\<tau>"
- | Unit
+ | TApp "term" "\<tau>"
+ | Ctor "ctor_name"
  | Lam x::"var" "\<tau>" e::"term" binds x in e  ("\<lambda> _ : _ . _" 50)
  | TyLam a::"tyvar" "\<kappa>" e::"term" binds a in e ("\<Lambda> _ : _ . _" 50)
  | Let x::"var" "\<tau>" "term" e2::"term" binds x in e2
 
 nominal_datatype "binder" =
-  "BVar" "var" "\<tau>"
-  | "BTyVar" "tyvar" "\<kappa>"
+  BVar "var" "\<tau>"
+  | BTyVar "tyvar" "\<kappa>"
+
+nominal_datatype "axiom" =
+  AxData "data_name" "\<kappa>"
+  | AxCtor "ctor_name" "\<tau>"
 
 type_synonym "\<Gamma>" = "binder list"
+type_synonym "\<Delta>" = "axiom list"
 
 lemma no_vars_in_kinds[simp]: "atom (x :: var) \<sharp> (k :: \<kappa>)"
   by (induction k rule: \<kappa>.induct) auto
 lemma no_vars_in_ty[simp]: "atom (x :: var) \<sharp> (ty :: \<tau>)"
-  by (induction ty rule: \<tau>.induct) auto
+  by (induction rule: \<tau>.induct) auto
+lemma no_vars_in_axioms[simp]: "atom (x :: var) \<sharp> (\<Delta> :: \<Delta>)"
+proof (induction \<Delta>)
+  case (Cons a \<Delta>)
+  then show ?case by (cases a rule: axiom.exhaust) (auto simp: fresh_Cons)
+qed (rule fresh_Nil)
+
+lemma perm_axioms_vars[simp]: "((a::var) \<leftrightarrow> b) \<bullet> (\<Delta>::\<Delta>) = \<Delta>"
+  using flip_fresh_fresh by force
+lemma perm_\<tau>_vars[simp]: "((a::var) \<leftrightarrow> b) \<bullet> (\<tau>::\<tau>) = \<tau>"
+  using flip_fresh_fresh by force
 
 lemma no_tyvars_in_kinds[simp]: "atom (a :: tyvar) \<sharp> (k :: \<kappa>)"
   by (induction k rule: \<kappa>.induct) auto
 
 lemma supp_empty_kinds[simp]: "supp (k :: \<kappa>) = {}"
   by (induction k rule: \<kappa>.induct) (auto simp: \<kappa>.supp)
+
+lemma perm_data_name_var[simp]: "((a::var) \<leftrightarrow> b) \<bullet> (T :: data_name) = T"
+  using flip_fresh_fresh by force
+lemma perm_data_name_tyvar[simp]: "((a::tyvar) \<leftrightarrow> b) \<bullet> (T :: data_name) = T"
+  using flip_fresh_fresh by force
+lemma perm_ctor_name_var[simp]: "((a::var) \<leftrightarrow> b) \<bullet> (D :: ctor_name) = D"
+  using flip_fresh_fresh by force
+lemma perm_ctor_name_tyvar[simp]: "((a::tyvar) \<leftrightarrow> b) \<bullet> (D :: ctor_name) = D"
+  using flip_fresh_fresh by force
 
 end
